env_subst.v
@@ -1,0 +1,63 @@
+Require Import reg_nar_lemmas.
+
+(** Les variables avec les noms suivants prennent le type correspondant par défaut : *)
+
+Implicit Types 
+(x y z X Y Z : nat)
+(T U V : typ)
+(n k p q : kind)
+(t s u v : term)
+(e f : env).
+
+Inductive env_subst T : nat -> env -> env -> Prop :=
+| snil e k : env_subst T 0 ((etvar k)::e) e
+| styp n e e' U : env_subst T n e e' -> env_subst T n (evar T :: e) (evar (tsubst U T n) :: e')
+| skind n e e' k : env_subst T n e e' -> env_subst T (S n) (etvar k :: e) (etvar k :: e').
+
+Lemma env_subst_wf_typ E1 E2 X T T2 :
+  wf_typ E1 T2 ->
+  wf_env E1 ->
+  env_subst T X E1 E2 ->
+  wf_env E2 ->
+  wf_typ E2 (tsubst T2 T X).
+Proof.
+  admit.
+Qed.
+
+Lemma env_subst_wf_env E1 E2 X T : 
+  wf_env E1 ->
+  env_subst T X E1 E2 ->
+  wf_env E2.
+Proof.
+  admit.
+Qed.
+
+Lemma env_subst_kinding E1 E2 T1 T2 X T k : 
+  env_subst T1 X E1 E2 ->
+  kinding E1 T2 k ->
+  kinding E2 (tsubst T2 T1 X) k.
+Proof.
+  admit.
+Qed.
+
+Lemma env_subst_typing E1 E2 T1 T2 t X : 
+  env_subst T1 X E1 E2 ->
+  typing E1 t T2 ->
+  typing E2 (subst_type t T1 X) T2.
+Proof.
+  admit.
+Qed.
+
+
+(* ??? *
+Fixpoint replace_var e n p := match e with
+| nil => nil
+| d::e' => match n with
+  | 0 => match d with
+    | etvar q => (etvar p)::e'
+    | d => d::e'
+    end
+  | S n' => d::(replace_var e' n p)
+  end
+
+*)
